lookup functional

src/extensions/paths/Lookup.v
@@ -20,7 +20,7 @@ Require Import Definitions Binding.
 (** Looking up a path in a stack (generalization of variable binding). *)
 
 Reserved Notation "s '∋' t" (at level 40).
-Reserved Notation "s '⟦' p '⟼' t '⟧'" (at level 40).
+Reserved Notation "s '⟦' t '⟼' u '⟧'" (at level 40).
 Reserved Notation "s '↓' p '==' ds" (at level 40).
 
 Inductive lookup_step : sta -> trm -> trm -> Prop :=
@@ -56,9 +56,11 @@ with lookup_open : sta -> path -> defs -> Prop :=
 
 where "s '↓' p '==' ds" := (lookup_open s p ds).
 
+Notation "s '⟦' t '⟼*' u '⟧'" := (star (lookup_step s) t u) (at level 40).
+
 Inductive lookup : sta -> path * val -> Prop :=
 | lookup_def: forall s p v,
-    star (lookup_step s) (trm_path p) (trm_val v) ->
+    s ⟦ trm_path p ⟼* trm_val v ⟧ ->
     s ∋ (p, v)
 
 where "s '∋' t" := (lookup s t).
@@ -70,47 +72,6 @@ Scheme lookup_mut := Induction for lookup_step Sort Prop
 Combined Scheme lookup_mutind from lookup_mut, lookup_open_mut.
 
 (** ** Lemmas about Environment Lookup *)
-(*
-Lemma lookup_func_mut :
-  (forall s t,
-    s [[ p  t -> forall p v1 v2,
-    t = (p, v1) ->
-    s ∋ (p, v2) ->
-    v1 = v2) /\
-  (forall s p ds1,
-    s ↓ p == ds1 -> forall ds2,
-    s ↓ p == ds2 ->
-    ds1 = ds2).
-Proof.
-  apply lookup_mutind; intros.
-  - Case "lookup_var".
-    inversions H. dependent induction H0; unfolds sel_fields; try (destruct p; inversions x).
-    lets Hb: (binds_func b H). subst*.
-  - Case "lookup_val".
-    inversions H0. inversions H1; unfolds sel_fields, pvar; destruct p.
-    * inversion H0.
-    * destruct p0. inversions H0. specialize (H _ _ H4). subst. lets Hd: (defs_has_inv H6 d). inversion* Hd.
-    * inversions H0. destruct p0. inversions H2.
-      specialize (H _ _ H3). subst. lets Hd: (defs_has_inv H5 d). inversion Hd.
-  - Case "lookup_path".
-    inversions H1. inversions H2; unfolds sel_fields, pvar.
-    * destruct p. inversion H1.
-    * destruct p0, p. inversions H1. specialize (H _ _ H5). subst. lets Hd: (defs_has_inv H7 d). inversion Hd.
-    * destruct p0, p. inversions H1.  specialize (H _ _ H4). subst. lets Hd: (defs_has_inv H6 d). inversions Hd.
-      inversions l. inversions H4. apply* H0.
-  - Case "lookup_defs".
-    lets Hl: (lookup_defs l). inversions H0. specialize (H _ _ _ _ eq_refl H1).
-    inversion* H.
-Qed.
-
-Lemma lookup_func : forall s p v1 v2 ps1 ps2,
-    s ∋ (p, v1) // ps1 ->
-    s ∋ (p, v2) // ps2 ->
-    v1 = v2.
-Proof.
-  intros. lets Hl: (proj21 lookup_func_mut). specialize (Hl _ _ _ H _ _ _ _ eq_refl H0). apply Hl.
-Qed.
- *)
 
 Lemma lookup_empty_mut :
   (forall s t u,
@@ -264,14 +225,14 @@ Proof.
 
 
 Lemma lookup_val_inv: forall s v t,
-    star (lookup_step s) (trm_val v) t ->
+    s ⟦ trm_val v ⟼* t ⟧ ->
     t = trm_val v.
 Proof.
   introv Hs. dependent induction Hs. auto. inversion H.
 Qed.
 
 Lemma lookup_path_inv: forall s t p,
-    star (lookup_step s) t (trm_path p) ->
+    s ⟦ t ⟼* trm_path p ⟧ ->
     exists q, t = trm_path q.
 Proof.
   introv Hs. dependent induction Hs; eauto. destruct (IHHs _ eq_refl) as [q Heq]. subst.
@@ -280,7 +241,7 @@ Qed.
 
 Lemma lookup_last_path: forall s p v,
     s ∋ (p, v) ->
-    exists q, star (lookup_step s) (trm_path p) (trm_path q) /\
+    exists q, s ⟦ trm_path p ⟼* trm_path q ⟧ /\
          s ⟦ trm_path q ⟼ trm_val v ⟧.
 Proof.
   introv Hl.
@@ -290,4 +251,51 @@ Proof.
     exists r. split. eapply star_trans. apply star_one. apply  H. all: auto.
   - apply lookup_val_inv in H1. inversions H1.
     exists p. split*. apply star_refl.
+Qed.
+
+Lemma lookup_step_func_mut :
+  (forall s t t1,
+      s ⟦ t ⟼ t1 ⟧ -> forall t2,
+      s ⟦ t ⟼ t2 ⟧ ->
+      t1 = t2) /\
+  (forall s p ds1,
+    s ↓ p == ds1 -> forall ds2,
+    s ↓ p == ds2 ->
+    ds1 = ds2).
+Proof.
+  apply lookup_mutind; intros.
+  - Case "lookup_var".
+    inversions H. lets Hb: (binds_func b H2). subst*.
+    unfolds sel_fields. destruct p. inversion H0.
+  - Case "lookup_sel".
+    inversions H0; unfolds sel_fields; destruct p. inversion H1. destruct p0.
+    inversions H1. specialize (H _ H2). subst. apply* defs_has_inv.
+  - Case "lookup_defs".
+    lets Hl: (lookup_defs l). inversions H0. specialize (H _ H1). inversion* H.
+Qed.
+
+Lemma lookup_step_func: forall s t t1 t2,
+      s ⟦ t ⟼ t1 ⟧ ->
+      s ⟦ t ⟼ t2 ⟧ ->
+      t1 = t2.
+Proof.
+  intros. apply* lookup_step_func_mut.
+Qed.
+
+Lemma lookup_irred: forall s v,
+    irred (lookup_step s) (trm_val v).
+Proof.
+  inversion 1.
+Qed.
+
+Lemma lookup_func : forall s p v1 v2,
+    s ∋ (p, v1) ->
+    s ∋ (p, v2) ->
+    v1 = v2.
+Proof.
+  introv Hs1 Hs2.
+  lets H: (lookup_step_func). specialize (H s). inversions Hs1. inversions Hs2.
+  assert (irred (lookup_step s) (trm_val v1)) as Hirr1 by apply* lookup_irred.
+  assert (irred (lookup_step s) (trm_val v2)) as Hirr2 by apply* lookup_irred.
+  lets Hf: (finseq_unique H H2 Hirr1 H3 Hirr2). inversion* Hf.
 Qed.
